src/program_proof/buf/defs.v
@@ -1,0 +1,49 @@
+From RecordUpdate Require Import RecordSet.
+Import RecordSetNotations.
+
+
+From Perennial.program_proof Require Import proof_prelude.
+From Perennial.program_proof.addr Require Import specs.
+
+Definition inode_bytes := Z.to_nat 128.
+Definition inode_buf := vec u8 inode_bytes.
+Definition inode_to_vals {ext: ext_op} (i:inode_buf) : list val :=
+  fmap b2val (vec_to_list i).
+
+Inductive bufDataKind :=
+| KindBit
+| KindInode
+| KindBlock
+.
+
+Global Instance bufDataKind_eq_dec : EqDecision bufDataKind.
+Proof.
+  solve_decision.
+Defined.
+
+Inductive bufDataT : forall {K : bufDataKind}, Type :=
+| bufBit (b : bool) : @bufDataT KindBit
+| bufInode (i : inode_buf) : @bufDataT KindInode
+| bufBlock (b : Block) : @bufDataT KindBlock
+.
+
+Definition bufSz K : nat :=
+  match K with
+  | KindBit => 1
+  | KindInode => inode_bytes*8
+  | KindBlock => block_bytes*8
+  end.
+
+Record buf := {
+  bufKind : bufDataKind;
+  bufData : @bufDataT bufKind;
+  bufDirty : bool;
+}.
+
+Definition get_bit (b0 : u8) (off : u64) : bool :=
+  if decide (U8 1 = word.and (word.sru b0 (u8_from_u64 off)) (U8 1))
+  then true
+  else false.
+
+Definition valid_off K (off : u64) : Prop :=
+  int.val off `mod` bufSz K = 0.
